Abstract things correctly out

theories/Core/Semantic/ReadbackLemmas.v
@@ -1,27 +1,22 @@
 From Coq Require Import Lia PeanoNat Relations.
 From Mcltt Require Import Base Domain Evaluate EvaluateLemmas LibTactics Readback Syntax System.
 
-#[local]
-Definition functional_read_nf_prop s m M1 (_ : {{ Rnf m in s ↘ M1 }}) : Prop := forall M2 (Hread2: {{ Rnf m in s ↘ M2 }}), M1 = M2.
-#[local]
-Definition functional_read_ne_prop s m M1 (_ : {{ Rne m in s ↘ M1 }}) : Prop := forall M2 (Hread2 : {{ Rne m in s ↘ M2 }}), M1 = M2.
-#[local]
-Definition functional_read_typ_prop s m M1 (_ : {{ Rtyp m in s ↘ M1 }}) : Prop := forall M2 (Hread2 : {{ Rtyp m in s ↘ M2 }}), M1 = M2.
-Arguments functional_read_nf_prop /.
-Arguments functional_read_ne_prop /.
-Arguments functional_read_typ_prop /.
+Section functional_read.
+  Let functional_read_nf_prop s m M1 (_ : {{ Rnf m in s ↘ M1 }}) : Prop := forall M2 (Hread2: {{ Rnf m in s ↘ M2 }}), M1 = M2.
+  Let functional_read_ne_prop s m M1 (_ : {{ Rne m in s ↘ M1 }}) : Prop := forall M2 (Hread2 : {{ Rne m in s ↘ M2 }}), M1 = M2.
+  Let functional_read_typ_prop s m M1 (_ : {{ Rtyp m in s ↘ M1 }}) : Prop := forall M2 (Hread2 : {{ Rtyp m in s ↘ M2 }}), M1 = M2.
 
-Lemma functional_read_nf : forall {s m M1}, {{ Rnf m in s ↘ M1 }} -> forall M2 (Hread2: {{ Rnf m in s ↘ M2 }}), M1 = M2
-with functional_read_ne : forall {s m M1}, {{ Rne m in s ↘ M1 }} -> forall M2 (Hread2 : {{ Rne m in s ↘ M2 }}), M1 = M2
-with functional_read_typ : forall {s m M1}, {{ Rtyp m in s ↘ M1 }} -> forall M2 (Hread2 : {{ Rtyp m in s ↘ M2 }}), M1 = M2.
-Proof with mauto.
-  all: clear functional_read_nf functional_read_ne functional_read_typ; intros * Hread1.
-  - (* functional_read_nf *)
+  #[local]
+  Ltac unfold_functional_read := unfold functional_read_nf_prop, functional_read_ne_prop, functional_read_typ_prop in *.
+
+  Lemma functional_read_nf : forall s m M1 (Hread1: {{ Rnf m in s ↘ M1 }}), functional_read_nf_prop s m M1 Hread1.
+  Proof using Type with mauto .
+    intros *.
     induction Hread1
       using read_nf_mut_ind
       with (P0 := functional_read_ne_prop)
            (P1 := functional_read_typ_prop);
-      simpl in *; mauto;
+      unfold_functional_read; mauto;
       intros; inversion Hread2; clear Hread2; subst;
       try replace m'0 with m' in * by mauto;
       try replace b0 with b in * by mauto;
@@ -29,12 +24,16 @@ Proof with mauto.
       try replace bs0 with bs in * by mauto;
       try replace ms0 with ms in * by mauto;
       f_equal...
-  - (* functional_read_ne *)
+  Qed.
+
+  Lemma functional_read_ne : forall s m M1 (Hread1 : {{ Rne m in s ↘ M1 }}), functional_read_ne_prop s m M1 Hread1.
+  Proof using Type with mauto.
+    intros *.
     induction Hread1
       using read_ne_mut_ind
       with (P := functional_read_nf_prop)
            (P1 := functional_read_typ_prop);
-      simpl in *; mauto;
+      unfold_functional_read; mauto;
       intros; inversion Hread2; clear Hread2; subst;
       try replace m'0 with m' in * by mauto;
       try replace b0 with b in * by mauto;
@@ -42,12 +41,16 @@ Proof with mauto.
       try replace bs0 with bs in * by mauto;
       try replace ms0 with ms in * by mauto;
       f_equal...
-  - (* functional_read_typ *)
+  Qed.
+
+  Lemma functional_read_typ : forall s m M1 (Hread1 : {{ Rtyp m in s ↘ M1 }}), functional_read_typ_prop s m M1 Hread1.
+  Proof using Type with mauto.
+    intros *.
     induction Hread1
       using read_typ_mut_ind
       with (P := functional_read_nf_prop)
            (P0 := functional_read_ne_prop);
-      simpl in *; mauto;
+      unfold_functional_read; mauto;
       intros; inversion Hread2; clear Hread2; subst;
       try replace m'0 with m' in * by mauto;
       try replace b0 with b in * by mauto;
@@ -55,7 +58,8 @@ Proof with mauto.
       try replace bs0 with bs in * by mauto;
       try replace ms0 with ms in * by mauto;
       f_equal...
-Qed.
+  Qed.
+End functional_read.
 
 #[global]
 Hint Resolve functional_read_nf functional_read_ne functional_read_typ : mcltt.
